theories/kcas/kcas_2__code.v
@@ -1,0 +1,138 @@
+From zoo Require Import
+  prelude.
+From zoo.language Require Import
+  typeclasses
+  notations.
+From zoo Require Import
+  identifier.
+From zoo_std Require Import
+  lst.
+From kcas Require Import
+  kcas_2__types.
+From zoo Require Import
+  options.
+
+Definition kcas_status_to_bool : val :=
+  fun: "status" =>
+    "status" == §After.
+
+Definition kcas_finish : val :=
+  fun: "gid" "casn" "status" =>
+    match: "casn".{status} with
+    | Before =>
+        #false
+    | After =>
+        #true
+    | Undetermined <> as "old_status" =>
+        Resolve
+          (CAS "casn".[status] "old_status" "status")
+          "casn".{proph}
+          ("gid", kcas_status_to_bool "status") ;;
+        kcas_status_to_bool "casn".{status}
+    end.
+
+#[local] Definition __zoo_recs_0 := (
+  recs: "determine_as" "casn" "cass" =>
+    let: "gid" := Id in
+    match: "cass" with
+    | [] =>
+        kcas_finish "gid" "casn" §After
+    | "cas" :: "cass'" =>
+        let: "loc", "state" := "cas" in
+        let: "proph" := Proph in
+        let: "state'" := !"loc" in
+        if: "state" == "state'" then (
+          "determine_as" "casn" "cass'"
+        ) else if:
+           Resolve ("state".<before> != "get_as" "state'") "proph" ()
+         then (
+          kcas_finish "gid" "casn" §Before
+        ) else (
+          match: "casn".{status} with
+          | Before =>
+              #false
+          | After =>
+              #true
+          | Undetermined <> =>
+              if: CAS "loc".[contents] "state'" "state" then (
+                "determine_as" "casn" "cass'"
+              ) else (
+                "determine_as" "casn" "cass"
+              )
+          end
+        )
+    end
+  and: "get_as" "state" =>
+    if: "determine" "state".<casn> then (
+      "state".<after>
+    ) else (
+      "state".<before>
+    )
+  and: "determine" "casn" =>
+    match: "casn".{status} with
+    | Before =>
+        #false
+    | After =>
+        #true
+    | Undetermined "cass" =>
+        "determine_as" "casn" "cass"
+    end
+)%zoo_recs.
+Definition kcas_determine_as :=
+  ValRecs 0 __zoo_recs_0.
+Definition kcas_get_as :=
+  ValRecs 1 __zoo_recs_0.
+Definition kcas_determine :=
+  ValRecs 2 __zoo_recs_0.
+#[global] Instance :
+  AsValRecs' kcas_determine_as 0 __zoo_recs_0 [
+    kcas_determine_as ;
+    kcas_get_as ;
+    kcas_determine
+  ].
+Proof.
+  done.
+Qed.
+#[global] Instance :
+  AsValRecs' kcas_get_as 1 __zoo_recs_0 [
+    kcas_determine_as ;
+    kcas_get_as ;
+    kcas_determine
+  ].
+Proof.
+  done.
+Qed.
+#[global] Instance :
+  AsValRecs' kcas_determine 2 __zoo_recs_0 [
+    kcas_determine_as ;
+    kcas_get_as ;
+    kcas_determine
+  ].
+Proof.
+  done.
+Qed.
+
+Definition kcas_make : val :=
+  fun: "v" =>
+    let: "_gid" := Id in
+    let: "casn" := { §After, Proph } in
+    let: "state" := Reveal ("casn", "v", "v") in
+    ref "state".
+
+Definition kcas_get : val :=
+  fun: "loc" =>
+    kcas_get_as !"loc".
+
+Definition kcas_cas : val :=
+  fun: "cass" =>
+    let: "casn" := { §After, Proph } in
+    let: "cass" :=
+      lst_map
+        (fun: "cas" =>
+           let: "loc", "before", "after" := "cas" in
+           let: "state" := Reveal ("casn", "before", "after") in
+           ("loc", "state"))
+        "cass"
+    in
+    "casn" <-{status} Reveal ‘Undetermined( "cass" ) ;;
+    kcas_determine_as "casn" "cass".
